theories/Syntax.v
@@ -495,6 +495,7 @@ Unset Elimination Schemes.
 Inductive wf_term : forall (m n:nat), term -> Prop :=
 | wf_bag :
   forall m n m' n'
+    (HN' : n' <= 1)
     (G : lctxt m) (D : lctxt n)
     (UG : forall x, x < m -> (G x) = 1)
     (UD : forall x, x < n -> (D x) = 2 \/ (D x) = 0)
